\documentclass{minimal}
\usepackage[utf8]{inputenc}

\addtolength{\topmargin}{-.2in}
\addtolength{\textheight}{1.75in}

\begin{document}
\begin{equation}
  \vdash(\varphi\to\psi)\to((\psi\to\chi)\to(\varphi\to\chi))
\end{equation}

\begin{equation}
  \vdash(\varphi\to(\psi\to\chi))\to(\psi\to(\varphi\to\chi))
\end{equation}

\begin{equation}
  \vdash\varphi\to(\neg\varphi\to\psi)
\end{equation}

\begin{equation}
  \vdash\neg\varphi\to(\varphi\to\psi)
\end{equation}

\begin{equation}
  \vdash\neg\neg\varphi\to\varphi
\end{equation}

\begin{equation}
  \vdash(\varphi\to\psi)\to(\neg\psi\to\neg\varphi)
\end{equation}

\begin{equation}
  \vdash\varphi\to\neg\neg\varphi
\end{equation}

\begin{equation}
  \vdash(\varphi\to\neg\varphi)\to\neg\varphi
\end{equation}

\begin{equation}
  \vdash\varphi\to(\neg\psi\to\neg(\varphi\to\psi))
\end{equation}

\begin{equation}
  \vdash\varphi\to(\varphi\vee\psi)
\end{equation}

\begin{equation}
  \vdash\psi\to(\varphi\vee\psi)
\end{equation}

\begin{equation}
  \vdash(\varphi\to\chi)\to[(\psi\to\chi)\to((\varphi\vee\psi)\to\chi)]
\end{equation}

\begin{equation}
  \vdash(\varphi\wedge\psi)\to\varphi
\end{equation}

\begin{equation}
  \vdash(\varphi\wedge\psi)\to\psi
\end{equation}

% 15
\begin{equation}
  \vdash(\chi\to\varphi)\to[(\chi\to\psi)\to(\chi\to(\varphi\wedge\psi))]
\end{equation}

\begin{equation}
  \vdash(\varphi\wedge\psi)\to(\psi\wedge\varphi)
\end{equation}

\begin{equation}
  \vdash\varphi\to(\psi\to(\varphi\wedge\psi))
\end{equation}

\begin{equation}
  \vdash[(\varphi\wedge\chi)\vee(\psi\vee\chi)]\to((\varphi\vee\psi)\wedge\chi)
\end{equation}

\begin{equation}
  \vdash(\chi\to\theta)\to[(\varphi\to(\psi\to\chi))\to(\varphi\to(\psi\to\theta))]
\end{equation}

% 20
\begin{equation}
  \vdash(\varphi\wedge(\psi\to\chi))\to((\varphi\wedge\psi)\to\chi)
\end{equation}

\begin{equation}
  \vdash[(\varphi\wedge\psi)\to\chi]\to[\varphi\to(\psi\to\chi)]
\end{equation}

\begin{equation}
  \vdash(\varphi\vee\psi)\to(\chi\to[(\varphi\wedge\chi)\vee(\psi\wedge\chi)]
\end{equation}

\begin{equation}
  \vdash[(\varphi\vee\psi)\wedge\chi]\to[(\varphi\wedge\chi)\vee(\psi\wedge\chi)]
\end{equation}

\begin{equation}
  \vdash(\varphi\wedge\neg\varphi)\to\psi
\end{equation}

\begin{equation}
  \vdash\psi\to(\varphi\vee\neg\varphi)
\end{equation}

\end{document}
